Add perform_call demo.

Examples/funccalls/call_test_proofs.v
@@ -15,30 +15,75 @@ Require Import nops_o_rec_nop_armv8.
 Require Import nops_o_short_nop_armv8.
 Require Import nops_o_tail_nop_armv8.
 Require Import nops_o_tiny_nop_armv8.
+Require Import branch_nop_proofs.
+Require Import clobber_ret_proofs.
+Require Import faith_ret_proofs.
+Require Import loop_nop_proofs.
+Require Import short_nop_proofs.
+Require Import tail_nop_proofs.
+Require Import tiny_nop_proofs.
+
 
 
 Import ARM8Notations.
 Open Scope N.
 
-Definition funcs := [branch_nop;
-call_test;
-clobber_ret;
-faith_ret;
-loop_nop;
-rec_nop;
-short_nop;
-tail_nop;
-tiny_nop].
+Definition funcs := [
+    tiny_nop;
+    short_nop;
+    branch_nop;
+    loop_nop;
+    rec_nop;
+    tail_nop;
+    clobber_ret;
+    faith_ret;
+    call_test
+    ].
 
+Fixpoint combine_programs (ps: list program) s a : option (N*stmt) :=
+ match ps with
+ | nil => None
+ | p::ps => match p s a with
+            | Some x => Some x
+            | None => combine_programs ps s a
+            end
+  end.
 
-(* I'd like to use Picinae_theory.updateall to combine the programs,
-   but update all is expecting functions like 'A -> option B' whereas
-   programs are 'store -> addr -> option B'. 
-   Not sure what the cleanest way to do this is. *)
-Definition unstored_funcs := funcs.
+Definition whole_binary := combine_programs funcs.
+Theorem whole_binary_welltyped: welltyped_prog arm8typctx whole_binary. Proof. Picinae_typecheck. Qed.
 
-Definition call_test_combined :=
-  List.fold_left (updateall) funcs (fun _ => None).
+Theorem funcs_pfsub:
+  forall s f (F: In f funcs), f s ⊆ whole_binary s.
+Proof.
+  intro s. rewrite <-Forall_forall.
+  (* Trouble automating this part - `intros x y` yields "No product even after head reduction." *)
+  (*
+  apply Forall_cons;
+    unfold tiny_nop, whole_binary, combine_programs, funcs, pfsub;
+    unfold tiny_nop, short_nop, branch_nop, loop_nop, rec_nop, tail_nop, clobber_ret, faith_ret, call_test;
+    intros x y; destruct x;[discriminate|repeat (discriminate || assumption || destruct p as [p|p|])].
+  *)
+  Ltac unfold_all :=
+    unfold whole_binary, combine_programs, funcs, pfsub,
+           tiny_nop, short_nop, branch_nop, loop_nop, 
+           rec_nop, tail_nop, clobber_ret, faith_ret, call_test.
+  Ltac prove_pfsub x :=
+    destruct x as [|p]; [
+        discriminate
+      | repeat (discriminate || assumption || destruct p as [p|p|])].
+  apply Forall_cons; unfold_all. intros x y a. prove_pfsub x.
+  apply Forall_cons; unfold_all. intros x y a. prove_pfsub x.
+  apply Forall_cons; unfold_all. intros x y a. prove_pfsub x.
+  apply Forall_cons; unfold_all. intros x y a. prove_pfsub x.
+  apply Forall_cons; unfold_all. intros x y a. prove_pfsub x.
+  apply Forall_cons; unfold_all. intros x y a. prove_pfsub x.
+  apply Forall_cons; unfold_all. intros x y a. prove_pfsub x.
+  apply Forall_cons; unfold_all. intros x y a. prove_pfsub x.
+  apply Forall_cons; unfold_all. intros x y a. prove_pfsub x.
+  apply Forall_nil. 
+
+Qed.
+
 Definition call_test_exit (t:trace) :=
   match t with (Addr a, _)::_ => match a with
   | 0x001000cc => true
@@ -54,7 +99,7 @@ Theorem call_test_pc :
   forall s t x' s'
      (ENTRY: startof t (x',s') = (Addr 0x00100084,s))
      (MDL: models arm8typctx s),
-     satisfies_all call_test (call_test_invs s) call_test_exit ((x',s')::t).
+     satisfies_all whole_binary (call_test_invs s) call_test_exit ((x',s')::t).
 Proof.
   Local Ltac step := time arm8_step.
   intros. 
@@ -64,17 +109,45 @@ Proof.
   (* Inductive step *)
   intros.
   eapply startof_prefix in ENTRY; try eassumption.
-  eapply preservation_exec_prog in MDL; try (eassumption || apply calltest_welltyped).
+  eapply preservation_exec_prog in MDL; try (eassumption || apply whole_binary_welltyped).
   clear - PRE MDL. rename t1 into t. rename s into s0; rename s1 into s.
   destruct_inv 64 PRE.
   rename PRE into S0.
-  step. step. step.
-  repeat step.
-  
-  repeat step; unfold arm8equiv in *; intros v SIG; specialize (S0 v SIG).
-    destruct v; match goal with
-    | [ |- context[or (eq true true) _] ] => now left
-    | _ => repeat (rewrite update_updated || rewrite update_frame); try easy
-    end.
-    now rewrite <-S0.
+  step. step.
+  (* We are at the entry of tiny_nop (0x00100000), so apply perform_call *)
+  remember (update (update s R_X0 (VaN n 64)) R_X30 (VaN 1048716 64)) as current_s.
+  apply perform_call with (Invs2:=tiny_nop_invs current_s) (xp2:=tiny_nop_exit); try reflexivity.
+    intros; unfold tiny_nop_exit. destruct (N.eq_dec a 1048576).
+      subst. unfold whole_binary, combine_programs, funcs, tiny_nop in H. discriminate.
+      clear - n0. destruct a.
+        reflexivity.
+        time repeat (reflexivity || contradiction || destruct p as [p|p|]).
+    intro t'. unfold effinv_impl,effinv. rewrite Bool.orb_true_l, Bool.orb_true_l.
+      unfold tiny_nop_invs, tiny_nop_exit, call_test_invs, call_test_exit.
+      destruct t' as [|x_s t'];[easy|destruct x_s as [x s']]. destruct x; try easy.
+      destruct a eqn:EQa; try easy. repeat (easy || destruct p as [p|p|]).
+      (* Here we are asked to prove the invariants for call_test entry and exit
+         without any information.
+         The goal in focus is the call-test postcondition.
+         We're being asked to prove that the current store, s', of an arbitrary
+         trace matches our original store with some exceptions.
+         This seems impossible...
+       *) admit. admit.
+    intros; split; reflexivity.
+    intros. apply satall_pmono with (p1:=tiny_nop).
+      intro s1. apply (funcs_pfsub s1 tiny_nop). apply in_eq.
+      admit.
+      destruct xs' as [x' s']. apply tiny_nop_pc.
+        assumption.
+        admit. (* Punting on proving store's typesafety *)
+        
+  (* Great! We're ready to keep going assuming all of our admits,
+     ~~ including the impossible looking ones ~~
+     are provable.
+  *)
+     intros.
+     Print get_precondition.
+     Print get_postcondition.
+     Locate destruct_inv.
+     destruct_inv 64 PRE. step.
 Qed.
